Kura/Conn/Minor.lean
@@ -2,11 +2,11 @@ import Kura.Conn.Conn
 
 namespace Graph
 open edge
-variable {V W E F : Type*} [DecidableEq V] [DecidableEq W] (G : Graph V E) (e : E) (u v w : V)
+variable {V W E F : Type*} [DecidableEq V] [DecidableEq W] (G : Graph V E)
 
 
 -- Merges to the start of the path
-def Mp (G : Graph V E) [DecidableEq E] (P : G.Path) :
+def Mpath (P : G.Path) :
     Graph {v : V // v ∉ P.vertices.tail} {e : E // e ∉ P.edges} where
   inc e := G
     |>.Qs {v : V | v ∈ P.vertices.tail} P.start P.start_not_mem_vertices_tail
@@ -15,14 +15,44 @@ def Mp (G : Graph V E) [DecidableEq E] (P : G.Path) :
 
 -- contraction by a rooted forest?
 
-structure MinorOf (G : Graph V E) (H : Graph W F) [DecidableEq E] [DecidableEq F] where
+structure MinorOf (H : Graph W F) where
   fw : W → Option V
   fₑ : E ↪ F
   comm : ∀ e : E, (H.inc (fₑ e)).map fw = (G.inc e).map some
-  connPreimage : ∀ (w₁ w₂ : W), fw w₁ = fw w₂ → H{(Set.range fₑ)ᶜ}ᴳ.conn w₁ w₂
+  connPreimage : ∀ (w₁ w₂ : W), fw w₁ = fw w₂ → (fw w₁).isSome → H{(Set.range fₑ)ᶜ}ᴳ.conn w₁ w₂
 
 
-def MinorOf.refl (G : Graph V E) [DecidableEq E] : G.MinorOf G := sorry
+def MinorOf.refl : G.MinorOf G where
+  fw := some
+  fₑ := Function.Embedding.refl E
+  comm _ := rfl
+  connPreimage u v huv _hSome := by
+    simp only [Option.some.injEq] at huv
+    subst huv
+    exact conn_refl _ u
 
-def MinorOf.OfSubgraph (G : Graph V E) (H : Graph W F) [DecidableEq E] [DecidableEq F]
-  (hGH : G ⊆ᴳ H) : G.MinorOf H := sorry
+noncomputable def MinorOf.OfSubgraph {G : Graph V E} {H : Graph W F} (hGH : G ⊆ᴳ H) :
+    G.MinorOf H where
+  fw w := by
+    by_cases hw : w ∈ Set.range hGH.fᵥ
+    · exact some (hGH.fᵥ.rangeSplitting ⟨w, hw⟩)
+    · exact none
+  fₑ := hGH.fₑ
+  comm e := by
+    simp only [Set.mem_range, hGH.comm, ← map_comp]
+    congr
+    ext u v
+    simp only [Set.mem_range, Function.comp_apply, EmbeddingLike.apply_eq_iff_eq, exists_eq,
+      ↓reduceDIte, Function.Embedding.rangeSplitting_apply, Option.mem_def, Option.some.injEq]
+  connPreimage u v huv hSome := by
+    simp only [Set.mem_range, Option.isSome_dite] at hSome huv
+    obtain ⟨w, rfl⟩ := hSome
+    simp only [Set.mem_range, EmbeddingLike.apply_eq_iff_eq, exists_eq, ↓reduceDIte,
+      Function.Embedding.rangeSplitting_apply] at huv
+    by_cases hv : v ∈ Set.range hGH.fᵥ
+    · simp only [hv, ↓reduceDIte, Option.some.injEq] at huv
+      subst huv
+      simp only [Function.Embedding.rangeSplitting_eq_val, conn_refl]
+    · simp only [hv, ↓reduceDIte, reduceCtorEq] at huv
+
+
