Kura/Planarity/Plainarity.lean
@@ -135,7 +135,7 @@ lemma EulerFormula_aux [Nonempty V] [Fintype V] [Fintype E]:
     let G' := G{{e}ᶜ}ᴳ
     have hG'Undir : G'.Undirected := by sorry
     have hG'Planar : Planar_by_AbstractDual G' := by sorry
-    -- let hG'SubgraphOf : G'.SubgraphOf G :=
+    let hSubgraph : G'.SubgraphOf G := Es_subgraph G {e}ᶜ
     specialize @ih ({e}ᶜ : Set E) _ G' hG'Undir hG'Planar _ (by simp only [compl,
       Set.mem_singleton_iff, Set.coe_setOf, Fintype.card_subtype_compl, hEcard,
       Fintype.card_ofSubsingleton, add_tsub_cancel_right])
@@ -148,17 +148,42 @@ lemma EulerFormula_aux [Nonempty V] [Fintype V] [Fintype E]:
       1 + G.NumberOfComponents + Fintype.card G'.Faces by
       omega
 
-    obtain u := G.v1 e
-    obtain v := G.v2 e
+    let u := G.v1 e
+    let v := G.v2 e
     by_cases hG'conn : G'.conn u v
     · have hNC : G'.NumberOfComponents = G.NumberOfComponents := by
         unfold Graph.NumberOfComponents
         have hconnEq : G'.connSetoid = G.connSetoid := by
           ext x y
           simp only [Setoid.Rel, Graph.connSetoid]
-          have hadj : G'.adj ≤ G.adj := sorry
+          have hadj : G'.adj ≤ G.adj := by
+            intro a b hSub
+            have := hSubgraph.Adj a b hSub
+            unfold_let at this
+            simpa only [Es_subgraph_fᵥ, id_eq] using this
           have hconn : G'.conn ≤ G.conn := Relation.ReflTransClosure.monotone hadj
-          have hadj' : G.adj ≤ G'.conn := sorry
+          have hadj' : G.adj ≤ G'.conn := by
+            rintro a b h
+            obtain ⟨e', he'⟩ := h
+            by_cases h : e' = e
+            · subst e'
+              simp only [canGo, inc_eq_undir_v12, edge.canGo_iff_eq_of_undir, Sym2.eq,
+                Sym2.rel_iff', Prod.mk.injEq, Prod.swap_prod_mk] at he'
+              rcases he' with ⟨rfl, rfl⟩ | ⟨rfl, rfl⟩
+              · change G'.conn u v
+                assumption
+              · change G'.conn v u
+                rw [conn_comm]
+                assumption
+            · have : G'.adj a b := by
+                let e'' : ({e}ᶜ : Set E) := ⟨e', by simp only [Set.mem_compl_iff,
+                  Set.mem_singleton_iff, h, not_false_eq_true]⟩
+                use e''
+                have := hSubgraph.canGo_iff a b e''
+                rw [Es_subgraph_fᵥ, Es_subgraph_fₑ, id_eq, id_eq] at this
+                rw [this]
+                exact he'
+              exact Relation.ReflTransGen.single this
           have hconn' : G.conn ≤ G'.conn := by
             conv_rhs =>
               change Relation.ReflTransClosure G'.adj
